Test_ReTierDynamicSemantics.v
@@ -275,9 +275,228 @@ Example testSubst_peerApp_1:
   = (peerApp (PeerInst 0)).
 Proof. reflexivity. Qed.
 
-
+(*
 Example testSubst_remoteApp_1:
   [(Id "x") := (some unit)]
   (remoteApp (remoteInst 0))
   = (remoteApp (remoteInst 0)).
 Proof. reflexivity. Qed.
+*)
+
+
+
+(* ====================================================================
+   Tests for implementation of pull based reactive system:
+*)
+Definition testR1V1 := (some unit).
+Definition testR2V1 := (none Unit).
+Definition testReactSys_p_1 := reactAlloc testR1V1 emptyReactSys.
+Definition testReactSys_p_2 := reactAlloc testR2V1 (snd testReactSys_p_1).
+
+Example testReactAlloc_1:
+  match testReactSys_p_1 with
+  | (r1, ReactiveSystem _ _ map) => map r1
+  end
+  = Some (some unit).
+Proof.
+  reflexivity.
+Qed.
+
+Example testReactAlloc_2:
+  match testReactSys_p_1 with
+  | (r1, _) =>  match testReactSys_p_2 with
+                | (r2, ReactiveSystem _ _ map) => (map r1, map r2)
+                end
+  end
+  = (Some (some unit), Some (none Unit)).
+Proof.
+  reflexivity.
+Qed.
+
+(* tests for 'curentValue' implicity also test 'reactAlloc' *)
+Definition testCurrentValue_1:
+  currentValue (fst testReactSys_p_1) (snd testReactSys_p_1) = (Some testR1V1, (snd testReactSys_p_1)).
+Proof. reflexivity. Qed.
+
+Definition testCurentValue_2:
+  currentValue (fst testReactSys_p_2) (snd testReactSys_p_2) = (Some testR2V1, (snd testReactSys_p_2)).
+Proof. reflexivity. Qed.
+
+Definition testCurentValue_3:
+  currentValue (Reactive 99) (snd testReactSys_p_2) = (None,  (snd testReactSys_p_2)).
+Proof. reflexivity. Qed.
+
+Definition testR1V2 := (lambda (Id "x") (*:*) Unit (*.*) unit).
+Definition testReactSys_3 := updateVar (fst testReactSys_p_1) testR1V2 (snd testReactSys_p_2).
+
+Example testUpdateVar_1:
+  currentValue (fst testReactSys_p_1) testReactSys_3 = (Some testR1V2, testReactSys_3).
+Proof. reflexivity. Qed.
+
+Example testUpdateVar_2:
+  currentValue (fst testReactSys_p_2) testReactSys_3 = (Some testR2V1, testReactSys_3).
+Proof. reflexivity. Qed.
+
+
+
+(* ====================================================================
+   Tests for relation 'localStep':
+*)
+
+
+Definition testTies1  :=  (tie_update (Peer "p0" *-> Peer "pm")
+                            (tie_update (Peer "p0" ?-> Peer "po")
+                              (tie_update (Peer "p0" S-> Peer "ps")
+                                (tie_update ((Peer "p0") N-> (Peer "pn"))
+                                  noTies)))).
+Definition testPeerTyping1 := (pT_update (PeerInst 4) (Peer "pm")
+                                (pT_update (PeerInst 3) (Peer "po")
+                                  (pT_update (PeerInst 2) (Peer "ps")
+                                    (pT_update (PeerInst 1) (Peer "pn")
+                                      (pT_update (PeerInst 0) (Peer "p0")
+                                      noPeers))))).
+Definition testPeerInsts1 := (pISet_add (PeerInst 4)
+                                (pISet_add (PeerInst 3)
+                                  (pISet_add (PeerInst 2)
+                                    (pISet_add (PeerInst 1)
+                                      (pISet_add (PeerInst 0)
+                                        noPeerInsts))))).
+Definition testTies1Context := LeContext testTies1 testPeerTyping1 testPeerInsts1 (Peer "p0") emptyReactSys.
+
+Example testLocalStep_EApp_1:
+  emptyLeContext |> (app (lambda (Id "x") (Option Unit) (unit)) (some unit)) L==> Right _ _ unit.
+Proof. apply E_App. Qed.
+
+Example testLocalStep_EApp_2:
+  emptyLeContext |> (app (lambda (Id "x") (Option Unit) (idApp (Id "x")))) (some unit)
+    L==> Right _ _ (some unit).
+Proof. apply E_App. Qed.
+
+
+Example testLocalStep_EAsLocal_1:
+  testTies1Context |> (asLocal unit (*:*) (Unit on (Peer "ps"))) L==> Right _ _ unit.
+Proof.
+  eapply E_AsLocal.
+  - reflexivity.
+  - reflexivity.
+  - reflexivity.
+Qed.
+
+
+Example testLocalStep_EComp_1:
+  testTies1Context |> asLocalIn (Id "x") (*=*) unit (*in*)  (idApp (Id "x")) (*:*) (Unit on (Peer "ps"))
+    L==> Right _ _ (asLocal unit (*:*) (Unit on (Peer "ps"))).
+Proof. apply E_Comp. Qed.
+
+
+Example testLocalStep_ERemote_1:
+  testTies1Context |> asLocal (app (lambda (Id "x") (Option Unit) (unit)) (some unit)) (*:*) (Unit on (Peer "ps"))
+    L==> Right _ _ (asLocal unit (*:*) (Unit on (Peer "ps"))).
+Proof.
+  eapply E_Remote.
+  - reflexivity.
+  - reflexivity.
+  - apply E_App.
+Qed.
+
+
+Example testLocalStep_EAsLocalFrom_1:
+  testTies1Context |> asLocalFrom unit (*:*) (Unit on (Peer "ps")) (*from*) (peerApp (PeerInst 2))
+    L==> Right _ _ unit.
+Proof. apply E_AsLocalFrom. Qed.
+
+
+Example testLocalStep_ECompFrom_1:
+  testTies1Context |> asLocalInFrom (Id "x") (*=*) unit (*in*) (idApp (Id "x")) (*:*) (Unit on (Peer "ps")) (*from*) (peerApp (PeerInst 2))
+    L==> Right _ _ (asLocalFrom unit (*:*) (Unit on (Peer "ps")) (*from*) (peerApp (PeerInst 2))).
+Proof. apply E_CompFrom. Qed.
+
+
+Example testLocalStep_ERemoteFrom_1:
+  testTies1Context |> asLocalFrom (app (lambda (Id "x") (Option Unit) (unit)) (some unit)) (*:*) (Unit on (Peer "ps")) (*from*) (peerApp (PeerInst 2))
+  L==> Right _ _ (asLocalFrom unit (*:*) (Unit on (Peer "ps")) (*from*) (peerApp (PeerInst 2))).
+Proof.
+  eapply E_RemoteFrom.
+  - reflexivity.
+  - reflexivity.
+  - apply E_App.
+Qed.
+  
+
+(* Tests for reactive rules *)
+
+Definition setReactiveSys (cont: leContext) (sys: reactiveSystem): leContext :=
+  match cont with
+  | LeContext ties peers peerInsts currentPeerT _ => LeContext ties peers peerInsts currentPeerT sys
+  end.
+
+Definition testReactSys_var1_p := reactAlloc (some unit) emptyReactSys.
+Definition testVar1 := fst testReactSys_var1_p.
+Definition testReactSys_var1 := snd testReactSys_var1_p.
+Example testLocalStep_EReactiveVar_1:
+  (* ensure test setup is correct ... *)
+  (match testReactSys_var1 with ReactiveSystem _ _ map => map testVar1 end)
+    = Some (some unit) /\
+  (* actual test ... *)
+  emptyLeContext ||> var (some unit) Ld==> Left _ _ testVar1, testReactSys_var1. 
+Proof.
+  split.
+  - reflexivity.
+  - eapply E_ReactiveVar. reflexivity.
+Qed.
+
+
+Definition testReactSys_var1_signal1_p := reactAlloc (reactApp testVar1) testReactSys_var1.
+Definition testSignal1 := fst testReactSys_var1_signal1_p.
+Definition testReactSys_var1_signal1 := snd testReactSys_var1_signal1_p.
+Definition testContext_var1 := setReactiveSys emptyLeContext testReactSys_var1.
+Example testLocalStep_ESignal_1:
+  testContext_var1 |> signal (reactApp testVar1) L==> Left _ _ testSignal1.
+Proof.
+  eapply E_Signal. reflexivity.
+Qed.
+
+
+Definition testContext_var1_signal1 := setReactiveSys emptyLeContext testReactSys_var1_signal1.
+Definition testReactSys_var1None := updateVar testVar1 (none Unit) testReactSys_var1.
+Example testLocalStep_ESet_1:
+  (* ensure test setup is correct ... *)
+  currentValue testVar1 (getReactSys testContext_var1) = (Some (some unit), testReactSys_var1) /\
+  currentValue testVar1 testReactSys_var1None  = (Some (none Unit), testReactSys_var1None) /\
+  (* actual test ... *)
+  testContext_var1 ||> set (reactApp testVar1) (*:=*) (none Unit) Ld==> (Right _ _ unit), testReactSys_var1None.
+Proof.
+  split.
+  - reflexivity.
+  - split.
+    + reflexivity.
+    + eapply E_Set. reflexivity.
+Qed.
+
+
+Definition testReactSys_var1None_signal1 := updateVar testVar1 (none Unit) testReactSys_var1_signal1.
+Definition testContext_var1None_signal1 := setReactiveSys emptyLeContext testReactSys_var1None_signal1.
+Example testLocalStep_ENow_1:
+  (* ensure test setup is correct ... *)
+  currentValue testVar1 (getReactSys testContext_var1_signal1) = (Some (some unit), testReactSys_var1_signal1) /\
+  (* actual test ... *)
+  testContext_var1_signal1 ||> now (reactApp testVar1) Ld==> Right _ _ (some unit), testReactSys_var1_signal1.
+Proof.
+  split.
+  - reflexivity.
+  - eapply E_Now. reflexivity.
+Qed.
+
+Example testLocalStep_ENow_2:
+  (* ensure test setup is correct ... *)
+  currentValue testVar1 (getReactSys testContext_var1_signal1) = (Some (some unit), testReactSys_var1_signal1) /\
+  currentValue testSignal1 (getReactSys testContext_var1_signal1) = (Some (reactApp testVar1), testReactSys_var1_signal1) /\
+  (* actual test ... *)
+  testContext_var1_signal1 ||> now (reactApp testVar1) Ld==> Right _ _ (some unit), testReactSys_var1_signal1.
+Proof.
+  split.
+  - reflexivity.
+  - split.
+    + reflexivity.
+    + eapply E_Now. reflexivity.
+Qed.
