ReTierProofTypePreservation.v
@@ -1,0 +1,155 @@
+Require Import ReTierSyntax.
+Require Import ReTierStaticSemantics.
+Require Import ReTierDynamicSemantics.
+Require Import ReTierProofSubstitution.
+Require Import ReTierProofAggregation.
+
+
+Lemma tied_not_None: forall context P1 P2,
+  areTied context P1 P2 = true -> getTieMult context (P1, P2) <> None.
+Proof.
+  intros context P1 P2. destruct context as [typing ties reacEnv placeEnv varEnv].
+  unfold areTied. simpl. destruct (ties (P1, P2)).
+  1-2: intros; congruence.
+Qed.
+
+Lemma tied_not_SomeMNone: forall context P1 P2,
+  areTied context P1 P2 = true -> getTieMult context (P1, P2) <> (Some mNone).
+Proof.
+  intros context P1 P2. destruct context as [typing ties reacEnv placeEnv varEnv].
+  unfold areTied. simpl. destruct (ties (P1, P2)).
+
+  1-2: unfold not; intros.
+  1: destruct m.
+  1-5: congruence.
+Qed.
+
+
+
+
+(* reminder:
+Inductive t : Type := 
+  | lambda : id -> T -> t -> t
+  | app    : t -> t -> t
+  | idApp  : id -> t
+  | unit   : t
+  | none   : T -> t
+  | some   : t -> t
+  | nil    : T -> t
+  | cons   : t -> t -> t
+  | asLocal       : t -> S -> t 
+  | asLocalFrom   : t -> S -> t -> t
+  | asLocalIn     : id -> t -> t -> S -> t
+  | asLocalInFrom : id -> t -> t -> S -> t -> t
+  | signal : t -> t
+  | var    : t -> t
+  | now    : t -> t
+  | set    : t -> t -> t
+  | peerApp          : p -> t
+  | reactApp      : r -> t
+  
+  (* Added to make testing easier. *)
+  | tnat   : nat -> t.
+
+(* static context *)
+Inductive context: Type :=
+  | Context: peerTyping -> Ties -> reactEnv -> placeEnv -> varEnv -> P -> context.
+
+(* dynamic context *)
+Inductive leContext: Type :=
+  | LeContext: Ties -> peerTyping -> peerInsts -> P -> reactiveSystem-> leContext.
+*)
+(*
+Lemma preservation_nonReactive: forall t t' T statContext dynContext,
+    statContext |- t \in T -> 
+    dynContext |> t L==> Right _ _ t' ->
+    exists T',
+    statContext |- t' \in T'.
+*)
+(* stronger formulation *)
+Lemma preservation_nonReactive: forall t t' T peerInsts typing ties reactEnv placeEnv varEnv P reactSys,
+    Context typing ties reactEnv placeEnv varEnv P |- t \in T -> 
+    LeContext ties typing peerInsts P reactSys |> t L==> Right _ _ t' ->
+    exists T',
+    Context typing ties reactEnv placeEnv varEnv P |- t' \in T'.
+Proof.
+  intros t t' T peerInsts typing ties reactEnv placeEnv varEnv P reactSys.
+  destruct t as [ x Tx body (* lambda : id -> T -> t -> t *)
+                | fct arg   (* app    : t -> t -> t *)
+                | x         (* idApp  : id -> t *)
+                |           (* unit   : t *)
+                | Tn        (* none   : T -> t *)
+                | ts        (* some   : t -> t *)
+                | Tn        (* nil    : T -> t *)
+                | tc tl     (* cons   : t -> t -> t *)
+                | targ S    (* asLocal       : t -> S -> t  *)
+                | targ S tfrom    (* asLocalFrom   : t -> S -> t -> t *)
+                | x tassign tin S (* asLocalIn     : id -> t -> t -> S -> t *)
+                | targ tassign tin S tfrom (* asLocalInFrom : id -> t -> t -> S -> t -> t *)
+                | ts        (* signal : t -> t *)
+                | tv        (* var    : t -> t *)
+                | tn        (* now    : t -> t *)
+                | ttarget tsource (* set    : t -> t -> t *)
+                | p         (* peerApp  : p -> t *)
+                | r         (* reactApp : r -> t *)
+                (* TODO: remove ? *)
+                | n         (* tnat   : nat -> t *)
+  ].
+  (* value cases,
+     i.e. cases in which no evaluation step is possible, because t is value *)
+    1,4-8,  (* cases  t = lambda x Tx body
+                      | unit
+                      | none Tn
+                      | some ts
+                      | nil Tn
+                      | cons tc tl *)
+    17-19,  (* cases  t = peerApp p
+                      | reactApp r
+                      | tnat n (* TODO: remove? *) *)
+  (* Left reactive cases,
+     i.e. cases in which no step is possible, because step would lead to Left _ _ t',
+     but Right _ _ t' is given *)
+    13-14,  (* cases  t = signal ts
+                      | var tv *)
+  (* variable case.
+     Cannot take evaluation step on variable, but case cannot occur since substitution
+     is applied before variable gets evaluated. *)
+    3:      (* case   t = idApp x *)
+      intros H_stat H_dyn; inversion H_dyn.
+  
+  Focus 2. (* t = asLocal targ S *)
+    intros H_stat H_dyn. destruct S as [Targ P1].
+    inversion H_stat. simpl in H2. rewrite H2 in H6, H7.
+    exists T.
+
+
+    (*destruct dynContext.*) inversion H_dyn. (* why does this create: asLocal t'0 ... ??? *)
+(*
+Focus 2.
+apply T_AsLocal with (P0 := P).
+1: reflexivity.
+2,3: assumption.
+*)
+
+    symmetry in H13. inversion H13. (* adds hypothesis ties = ties0 *)
+    rewrite H18, H21 in H16.
+    (* for lemma instantiation:
+        - p0 := P0
+        - p1 := P1
+        - peers := peers
+        - value := targ
+        - value_type := Targ
+    *)
+    apply aggregation with (p0 := P0) (p1 := P1) (peers := peers) (value := targ) (value_type := Targ).
+    1-4: rewrite H2.
+    3: simpl; symmetry.
+    3-5: assumption.
+    1: apply tied_not_None.
+    2: apply tied_not_SomeMNone.
+ 
+    1-2: assumption.
+    Focus 1. eapply T_AsLocal.
+    Focus 1. reflexivity.
+    2,3: simpl; assumption.
+    
+    Abort.
